lean-fx-2/LeanFX2/Algo/Soundness.lean
@@ -427,6 +427,8 @@ theorem Term.headStep?_sound
   | hcomp _ _ => nomatch firedEq
   | recordIntro _ => nomatch firedEq
   | recordProj _ => nomatch firedEq
+  | refineIntro _ _ _ => nomatch firedEq
+  | refineElim _ => nomatch firedEq
   | universeCode _ _ _ _ => nomatch firedEq
   | cumulUp _ _ _ _ _ _ => nomatch firedEq
   | equivReflId _ => nomatch firedEq
@@ -500,7 +502,7 @@ theorem Term.headStep?_sound
     | .interval0 | .interval1 | .intervalOpp | .intervalMeet | .intervalJoin
     | .pathLam | .pathApp
     | .glueIntro | .glueElim | .transp | .hcomp
-    | .recordIntro | .recordProj
+    | .recordIntro | .recordProj | .refineIntro | .refineElim
     | .universeCode | .cumulUp
     | .equivReflId | .funextRefl | .equivReflIdAtId | .funextReflAtId
     | .equivIntroHet | .equivApp | .uaIntroHet | .funextIntroHet
@@ -532,7 +534,7 @@ theorem Term.headStep?_sound
     | .interval0 | .interval1 | .intervalOpp | .intervalMeet | .intervalJoin
     | .pathLam | .pathApp
     | .glueIntro | .glueElim | .transp | .hcomp
-    | .recordIntro | .recordProj
+    | .recordIntro | .recordProj | .refineIntro | .refineElim
     | .universeCode | .cumulUp
     | .equivReflId | .funextRefl | .equivReflIdAtId | .funextReflAtId
     | .equivIntroHet | .equivApp | .uaIntroHet | .funextIntroHet
@@ -563,7 +565,7 @@ theorem Term.headStep?_sound
     | .interval0 | .interval1 | .intervalOpp | .intervalMeet | .intervalJoin
     | .pathLam | .pathApp
     | .glueIntro | .glueElim | .transp | .hcomp
-    | .recordIntro | .recordProj
+    | .recordIntro | .recordProj | .refineIntro | .refineElim
     | .universeCode | .cumulUp
     | .equivReflId | .funextRefl | .equivReflIdAtId | .funextReflAtId
     | .equivIntroHet | .equivApp | .uaIntroHet | .funextIntroHet
@@ -594,7 +596,7 @@ theorem Term.headStep?_sound
     | .interval0 | .interval1 | .intervalOpp | .intervalMeet | .intervalJoin
     | .pathLam | .pathApp
     | .glueIntro | .glueElim | .transp | .hcomp
-    | .recordIntro | .recordProj
+    | .recordIntro | .recordProj | .refineIntro | .refineElim
     | .universeCode | .cumulUp
     | .equivReflId | .funextRefl | .equivReflIdAtId | .funextReflAtId
     | .equivIntroHet | .equivApp | .uaIntroHet | .funextIntroHet
@@ -625,7 +627,7 @@ theorem Term.headStep?_sound
     | .interval0 | .interval1 | .intervalOpp | .intervalMeet | .intervalJoin
     | .pathLam | .pathApp
     | .glueIntro | .glueElim | .transp | .hcomp
-    | .recordIntro | .recordProj
+    | .recordIntro | .recordProj | .refineIntro | .refineElim
     | .universeCode | .cumulUp
     | .equivReflId | .funextRefl | .equivReflIdAtId | .funextReflAtId
     | .equivIntroHet | .equivApp | .uaIntroHet | .funextIntroHet
